is step_eq legit?

src/Init/Data/Iterators/Combinators/Monadic/Take.lean
@@ -66,7 +66,7 @@ This combinator incurs an additional O(1) cost with each output of `it`.
 -/
 @[always_inline, inline]
 def IterM.take [Iterator α m β] (n : Nat) (it : IterM (α := α) m β) :=
-  IterM.mk (Take.mk (n + 1) it (Or.inl <| Nat.zero_lt_succ _)) m β
+  (⟨Take.mk (n + 1) it (Or.inl <| Nat.zero_lt_succ _)⟩ : IterM m β)
 
 /--
 This combinator is only useful for advanced use cases.
@@ -92,14 +92,13 @@ This combinator incurs an additional O(1) cost with each output of `it`.
 -/
 @[always_inline, inline]
 def IterM.toTake [Iterator α m β] [Finite α m] (it : IterM (α := α) m β) :=
-  IterM.mk (Take.mk 0 it (Or.inr inferInstance)) m β
+  (⟨Take.mk 0 it (Or.inr inferInstance)⟩ : IterM m β)
 
 theorem IterM.take.surjective_of_zero_lt {α : Type w} {m : Type w → Type w'} {β : Type w}
     [Iterator α m β] (it : IterM (α := Take α m) m β) (h : 0 < it.internalState.countdown) :
     ∃ (it₀ : IterM (α := α) m β) (k : Nat), it = it₀.take k := by
   refine ⟨it.internalState.inner, it.internalState.countdown - 1, ?_⟩
-  simp only [take, Nat.sub_add_cancel (m := 1) (n := it.internalState.countdown) (by omega)]
-  rfl
+  simp [take, Nat.sub_add_cancel (m := 1) (n := it.internalState.countdown) (by omega)]
 
 namespace Iterators.Types
 
